\documentclass[11pt,twoside]{report}
\usepackage[a4paper,width=160mm,top=20mm,bottom=20mm,bindingoffset=6mm]{geometry}

\usepackage{amsfonts}
\usepackage{amsmath,amssymb}
\usepackage{graphicx}
\usepackage{wrapfig}
\usepackage[T1]{fontenc} 
\usepackage[utf8]{inputenc}
\usepackage{graphicx}
\usepackage{wrapfig}
\usepackage{mathtools} 
\usepackage{lipsum}
\usepackage{color}
\usepackage[english]{babel}
\usepackage{appendix}
\usepackage{float}
\usepackage{enumitem}
\usepackage{setspace}
\usepackage{subcaption}
\usepackage{amssymb}
\usepackage{fancyhdr}
\usepackage{titlesec}
\usepackage{mathrsfs}
\usepackage{fixmath}

\titleformat{\chapter}[display]
{\normalfont\huge\bfseries}{\chaptertitlename~\thechapter}{20pt}{\Huge}
\titlespacing*{\chapter}{0pt}{30pt}{15pt}
\titlespacing*{name=\chapter,numberless}{0pt}{-30pt}{10pt}

\newenvironment{system}
{\left\lbrace\begin{array}{*{4}{c@{}>{{}}c<{{}}@{}}c}}
	{\end{array}\right.}
\setlength{\parindent}{0pt}

\makeatletter
\@addtoreset{section}{part}
\makeatother
\renewcommand{\partname}{}
\linespread{0.75}
\newcommand\independent{\protect\mathpalette{\protect\independenT}{\perp}}
\def\independenT#1#2{\mathrel{\rlap{$#1#2$}\mkern2mu{#1#2}}}
\let\oldemptyset\emptyset
\let\emptyset\varnothing
\singlespacing
\newtheorem{definition}{Definition}
\newtheorem{lemma}{Lemma}

 
\begin{document}
\chapter{GCV}
\section{GCV-I-derivative}
$ \frac{dGCV}{d\lambda}(\lambda) = \frac{d(s\frac{SS_{res}(\lambda)}{dor^2(\lambda)})}{d\lambda} = s (\frac{dSS_{res}}{d\lambda}\frac{1}{dor^2} + SS_{res}\frac{d(dor^{-2})}{d\lambda}) $\\
\\
$[1] = \frac{dSS_{res}}{d\lambda} = \frac{d(<\hat{\mathbold{\varepsilon}},\hat{\mathbold{\varepsilon}}> )}{d\lambda} = 2<\frac{d\hat{\mathbold{\varepsilon}}}{d\lambda},\hat{\mathbold{\varepsilon}}> = 2 < \frac{d((\mathbold{Q}-\mathbold{Q}\mathbold{S})\mathbold{z})}{d\lambda}, \hat{\mathbold{\varepsilon}}> = -2<\mathbold{Q}\frac{d\mathbold{S}}{d\lambda}\mathbold{z}, \hat{\mathbold{\varepsilon}}> \overset{\mathbold{Q}\in Sym}{=}\\ -2<\frac{d\mathbold{S}}{d\lambda}\mathbold{z},\mathbold{Q} \hat{\mathbold{\varepsilon}}> \overset{\mathbold{Q}^2 = \mathbold{Q}}{=} -2<\frac{d\mathbold{S}}{d\lambda}\mathbold{z}, \hat{\mathbold{\varepsilon}}>$\\
\\
$[2]= \frac{d(dor^{-2})}{d\lambda} = -2\frac{1}{dor^3}\frac{d(dor)}{d\lambda} = -2\frac{1}{dor^3}\frac{d(s-q-tr(\mathbold{S}))}{d\lambda} = 2\frac{1}{dor^3}tr(\frac{d\mathbold{S}}{d\lambda})$\\
\\
$\implies \frac{dGCV}{d\lambda}(\lambda) = s (-<\frac{d\mathbold{S}}{d\lambda}\mathbold{z}, \hat{\mathbold{\varepsilon}}>\frac{2}{dor^2} + SS_{res}\frac{2}{dor^3}tr(\frac{d\mathbold{S}}{d\lambda})) = \frac{2s}{{dor}^2}(\hat{\sigma}^2tr(\frac{d\mathbold{S}}{d\lambda}) + a)$

\subsection{Fundamental matrices}
\begin{enumerate}
	\item $ \mathbf{R} = \mathbf{R_1}^t\mathbf{R_0}^{-1}\mathbf{R_1}$
	\item $ \mathbf{T} = \boldsymbol{\Psi}^t\mathbf{Q}\boldsymbol{\Psi}+\lambda\mathbf{R_1}^t\mathbf{R_0}^{-1}\mathbf{R_1} = \boldsymbol{\Psi}^t\mathbf{Q}\boldsymbol{\Psi}+\lambda\mathbf{R}$
	\item $\mathbf{V} = (\boldsymbol{\Psi}^t\mathbf{Q}\boldsymbol{\Psi}+\lambda\mathbf{R_1}^t\mathbf{R_0}^{-1}\mathbf{R_1})^{-1}\boldsymbol{\Psi}^t\mathbf{Q} = \boldsymbol{T}^{-1}\boldsymbol{\Psi}^t\mathbf{Q}$
	\item $ \mathbf{S} =  \boldsymbol{\Psi}(\boldsymbol{\Psi}^t\mathbf{Q}\boldsymbol{\Psi}+\lambda\mathbf{R_1}^t\mathbf{R_0}^{-1}\mathbf{R_1})^{-1}\boldsymbol{\Psi}^t\mathbf{Q} = \boldsymbol{\Psi}\boldsymbol{V}$
	\item $\frac{d\mathbold{S}}{d\lambda} = -\boldsymbol{\Psi}(\boldsymbol{\Psi}^t\mathbf{Q}\boldsymbol{\Psi}+\lambda\mathbf{R_1}^t\mathbf{R_0}^{-1}\mathbf{R_1})^{-1}\mathbf{R_1}^t\mathbf{R_0}^{-1}\mathbf{R_1}(\boldsymbol{\Psi}^t\mathbf{Q}\boldsymbol{\Psi}+\lambda\mathbf{R_1}^t\mathbf{R_0}^{-1}\mathbf{R_1})^{-1}\boldsymbol{\Psi}^t\mathbf{Q}\\
	= -\boldsymbol{\Psi}\mathbf{T}^{-1}\mathbf{R}\mathbf{V} = -\boldsymbol{\Psi}\mathbf{K}\mathbf{V} = -\boldsymbol{\Psi}\mathbf{F}$
\end{enumerate}


\paragraph{Useful stored factors}
\begin{enumerate}
	\item $\mathbf{K} = \mathbf{T}^{-1}\mathbf{R}$
	\item $\mathbf{F} = \mathbf{K}\mathbf{V}$
	\item $\mathbf{t} = \frac{d\mathbold{S}}{d\lambda}\mathbold{z}$
	\item $ a = -<\frac{d\mathbold{S}}{d\lambda}\mathbold{z}, \hat{\mathbold{\varepsilon}}> = -<\mathbf{t}, \hat{\mathbold{\varepsilon}}>$
\end{enumerate}
\newpage

\section{GCV-II-derivative}
$ \frac{d^2GCV}{d\lambda^2}(\lambda) = 2s\frac{d({dor}^{-2}(\hat{\sigma}^2tr(\frac{d\mathbold{S}}{d\lambda}) - <\frac{d\mathbold{S}}{d\lambda}\mathbold{z}, \hat{\mathbold{\varepsilon}}>))}{d\lambda}\\$
\\
$ [1] = \frac{d(dor^{-2})}{d\lambda}(\hat{\sigma}^2tr(\frac{d\mathbold{S}}{d\lambda}) - <\frac{d\mathbold{S}}{d\lambda}\mathbold{z}, \hat{\mathbold{\varepsilon}}>) =  2\frac{1}{dor^3}tr(\frac{d\mathbold{S}}{d\lambda})(\hat{\sigma}^2tr(\frac{d\mathbold{S}}{d\lambda}) - <\frac{d\mathbold{S}}{d\lambda}\mathbold{z}, \hat{\mathbold{\varepsilon}}>)$\\
\\
$ [2] = \frac{1}{dor^2}\frac{d(\hat{\sigma}^2)}{d\lambda}tr(\frac{d\mathbold{S}}{d\lambda}) = \frac{1}{dor^2}\frac{\frac{d(SS_{res})}{d\lambda}dor - SS_{res}\frac{d(dor)}{d\lambda}}{dor^2}tr(\frac{d\mathbold{S}}{d\lambda}) = \frac{1}{dor^2}\frac{-2<\frac{d\mathbold{S}}{d\lambda}\mathbold{z}, \hat{\mathbold{\varepsilon}}>dor + SS_{res}tr(\frac{d\mathbold{S}}{d\lambda})}{dor^2}tr(\frac{d\mathbold{S}}{d\lambda}) = \frac{1}{dor^3}(-2<\frac{d\mathbold{S}}{d\lambda}\mathbold{z}, \hat{\mathbold{\varepsilon}}> + \hat{\sigma}^2tr(\frac{d\mathbold{S}}{d\lambda}))tr(\frac{d\mathbold{S}}{d\lambda})$\\
\\
$ [3] =  \frac{1}{dor^2}\hat{\sigma}^2tr(\frac{d^2\mathbold{S}}{d\lambda^2})$\\
\\
$ [4] = - \frac{1}{dor^2}<\frac{d^2\mathbold{S}}{d\lambda^2}\mathbold{z}, \hat{\mathbold{\varepsilon}}>$\\
\\
$ [5] = - \frac{1}{dor^2}<\frac{d\mathbold{S}}{d\lambda}\mathbold{z}, \frac{d\hat{\mathbold{\varepsilon}}}{d\lambda}> = \frac{1}{dor^2}<\frac{d\mathbold{S}}{d\lambda}\mathbold{z},\mathbold{Q} \frac{d\mathbold{S}}{d\lambda}\mathbold{z}>$\\
\\
$\implies  \frac{d^2GCV}{d\lambda^2}(\lambda) =
\\ =\frac{2s}{dor^2}\{\frac{1}{dor}[3\hat{\sigma}^2tr(\frac{d\mathbold{S}}{d\lambda}) - 4<\frac{d\mathbold{S}}{d\lambda}\mathbold{z}, \hat{\mathbold{\varepsilon}}>]tr(\frac{d\mathbold{S}}{d\lambda}) + \hat{\sigma}^2tr(\frac{d^2\mathbold{S}}{d\lambda^2}) + <\frac{d\mathbold{S}}{d\lambda}\mathbold{z},\mathbold{Q} \frac{d\mathbold{S}}{d\lambda}\mathbold{z}> - <\frac{d^2\mathbold{S}}{d\lambda^2}\mathbold{z}, \hat{\mathbold{\varepsilon}}>\} = \\
=\frac{2s}{dor^2}\{\frac{1}{dor}[3\hat{\sigma}^2tr(\frac{d\mathbold{S}}{d\lambda}) + 4a]tr(\frac{d\mathbold{S}}{d\lambda}) + \hat{\sigma}^2tr(\frac{d^2\mathbold{S}}{d\lambda^2}) +b+c\}$

\subsection{Fundamental matrices}
\begin{enumerate}
	\item $\frac{d^2\mathbold{S}}{d\lambda^2} = 2 \boldsymbol{\Psi}[(\boldsymbol{\Psi}^t\mathbf{Q}\boldsymbol{\Psi}+\lambda\mathbf{R_1}^t\mathbf{R_0}^{-1}\mathbf{R_1})^{-1}\mathbf{R_1}^t\mathbf{R_0}^{-1}\mathbf{R_1}]^2(\boldsymbol{\Psi}^t\mathbf{Q}\boldsymbol{\Psi}+\lambda\mathbf{R_1}^t\mathbf{R_0}^{-1}\mathbf{R_1})^{-1}\boldsymbol{\Psi}^t\mathbf{Q}\\
	= 2\boldsymbol{\Psi}(\mathbf{T}^{-1}\mathbf{R})^2\mathbf{V} = 2\boldsymbol{\Psi}\mathbf{K}^2\mathbf{V} = 2\boldsymbol{\Psi}\mathbf{K}\mathbf{F}$
\end{enumerate}

\paragraph{Useful stored factors}
\begin{enumerate}
	\item $b = <\frac{d\mathbold{S}}{d\lambda}\mathbold{z},\mathbold{Q} \frac{d\mathbold{S}}{d\lambda}\mathbold{z}>  = <\mathbold{t},\mathbold{Q} \mathbold{t}>$
	\item $c = -<\frac{d^2\mathbold{S}}{d\lambda^2}\mathbold{z}, \hat{\mathbold{\varepsilon}}>$
\end{enumerate}

\chapter{Forced GCV}

\section{GCV-I-derivative}
$ \frac{dGCV}{d\lambda}(\lambda) = \frac{d(s\frac{SS_{res}(\lambda)}{dor^2(\lambda)})}{d\lambda} = s (\frac{dSS_{res}}{d\lambda}\frac{1}{dor^2} + SS_{res}\frac{d(dor^{-2})}{d\lambda}) $\\
\\
$[1] = \frac{dSS_{res}}{d\lambda} = \frac{d(<\hat{\mathbold{\varepsilon}},\hat{\mathbold{\varepsilon}}> )}{d\lambda} = 2<\frac{d\hat{\mathbold{\varepsilon}}}{d\lambda},\hat{\mathbold{\varepsilon}}> = 2 < \frac{d((\mathbold{Q}-\mathbold{Q}\mathbold{S})\mathbold{z}-\mathbf{r})}{d\lambda}, \hat{\mathbold{\varepsilon}}> = -2<\mathbold{Q}(\frac{d\mathbold{S}}{d\lambda}\mathbold{z} + \frac{d\mathbold{s}}{d\lambda}), \hat{\mathbold{\varepsilon}}> \overset{\mathbold{Q}\in Sym}{=}\\ -2<\frac{d\mathbold{S}}{d\lambda}\mathbold{z} + \frac{d\mathbold{s}}{d\lambda},\mathbold{Q} \hat{\mathbold{\varepsilon}}> \overset{\mathbold{Q}^2 = \mathbold{Q}}{=} 2<\lambda \boldsymbol{h} -(\frac{\mathbf{s}}{\lambda} +\mathbf{t}), \hat{\mathbold{\varepsilon}}> = 2a$\\
\\
$[2]= \frac{d(dor^{-2})}{d\lambda} = -2\frac{1}{dor^3}\frac{d(dor)}{d\lambda} = -2\frac{1}{dor^3}\frac{d(s-q-tr(\mathbold{S}))}{d\lambda} = 2\frac{1}{dor^3}tr(\frac{d\mathbold{S}}{d\lambda})$\\
\\
$\implies \frac{dGCV}{d\lambda}(\lambda) = s (\frac{2a}{dor^2} + SS_{res}\frac{2}{dor^3}tr(\frac{d\mathbold{S}}{d\lambda})) = \frac{2s}{{dor}^2}(\hat{\sigma}^2tr(\frac{d\mathbold{S}}{d\lambda}) + a)$

\paragraph{Useful side computations}
\begin{enumerate}
	\item $ \frac{d\mathbold{s}}{d\lambda} = \frac{\mathbf{s}}{\lambda} - \lambda \boldsymbol{\Psi} \textbf{T}^{-1} \textbf{R}\textbf{T}^{-1} \textbf{R}_1^T\textbf{R}_0^{-1}\textbf{u} =\frac{\mathbf{s}}{\lambda} - \lambda \boldsymbol{\Psi} \textbf{K}\mathbf{g} = \frac{\mathbf{s}}{\lambda} - \lambda \boldsymbol{\Psi} \textbf{k} = \frac{\mathbf{s}}{\lambda} - \lambda \boldsymbol{h} $
\end{enumerate}

\paragraph{Useful stored factors}
\begin{enumerate}
	\item $ \mathbf{f} = \textbf{R}_1^T\textbf{R}_0^{-1}\textbf{u} $
	\item $ \mathbf{g} = \textbf{T}^{-1}\textbf{f} $
	\item $ \mathbf{k} = \textbf{K}\mathbf{g}$
	\item $ \mathbf{h} = \boldsymbol{\Psi}\mathbf{k}$
	\item $ \mathbf{s} = \lambda \boldsymbol{\Psi} \textbf{T}^{-1} \textbf{R}_1^T\textbf{R}_0^{-1}\textbf{u} = \lambda \boldsymbol{\Psi}\mathbf{g} $
	\item $ \mathbf{r} = \lambda \textbf{Q}\boldsymbol{\Psi} \textbf{T}^{-1} \textbf{R}_1^T\textbf{R}_0^{-1}\textbf{u} = \lambda \textbf{Q}\boldsymbol{\Psi}\mathbf{g} = \textbf{Q}\mathbf{s}$
	\item $\mathbf{p} = \lambda \boldsymbol{h} -(\frac{\mathbf{s}}{\lambda} +\mathbf{t}) $
\end{enumerate}

\paragraph{Redefined factors}
\begin{enumerate}
	\item $ a = <\mathbf{p}, \hat{\mathbold{\varepsilon}}> $
\end{enumerate}

\newpage
\section{GCV-II-derivative}
$ \frac{d^2GCV}{d\lambda^2}(\lambda) = 2s\frac{d({dor}^{-2}(\hat{\sigma}^2tr(\frac{d\mathbold{S}}{d\lambda}) + <\mathbold{p}, \hat{\mathbold{\varepsilon}}>))}{d\lambda}\\$
\\
$ [1] = \frac{d(dor^{-2})}{d\lambda}(\hat{\sigma}^2tr(\frac{d\mathbold{S}}{d\lambda}) + <\boldsymbol{p}, \hat{\mathbold{\varepsilon}}>) =  2\frac{1}{dor^3}tr(\frac{d\mathbold{S}}{d\lambda})(\hat{\sigma}^2tr(\frac{d\mathbold{S}}{d\lambda}) + <\boldsymbol{p}, \hat{\mathbold{\varepsilon}}>)$\\
\\
$ [2] = \frac{1}{dor^2}\frac{d(\hat{\sigma}^2)}{d\lambda}tr(\frac{d\mathbold{S}}{d\lambda}) = \frac{1}{dor^2}\frac{\frac{d(SS_{res})}{d\lambda}dor - SS_{res}\frac{d(dor)}{d\lambda}}{dor^2}tr(\frac{d\mathbold{S}}{d\lambda}) = \frac{1}{dor^2}\frac{<\mathbold{p}, \hat{\mathbold{\varepsilon}}>dor + SS_{res}tr(\frac{d\mathbold{S}}{d\lambda})}{dor^2}tr(\frac{d\mathbold{S}}{d\lambda}) = \frac{1}{dor^3}(2<\mathbold{p}, \hat{\mathbold{\varepsilon}}> + \hat{\sigma}^2tr(\frac{d\mathbold{S}}{d\lambda}))tr(\frac{d\mathbold{S}}{d\lambda})$\\
\\
$ [3] =  \frac{1}{dor^2}\hat{\sigma}^2tr(\frac{d^2\mathbold{S}}{d\lambda^2})$\\
\\
$ [4] = \frac{1}{dor^2}<\frac{d\mathbold{p}}{d\lambda}, \hat{\mathbold{\varepsilon}}> =  \frac{1}{dor^2}<-\frac{d^2\mathbold{S}}{d\lambda^2}\mathbold{z} + \frac{\boldsymbol{s}}{\lambda^2} + \boldsymbol{h} + \lambda \frac{d\boldsymbol{h}}{d\lambda} - \frac{1}{\lambda}\frac{d\boldsymbol{s}}{d\lambda}, \hat{\mathbold{\varepsilon}}> =\\ \frac{1}{dor^2}<-\frac{d^2\mathbold{S}}{d\lambda^2}\mathbold{z} + \frac{\boldsymbol{s}}{\lambda^2} + \boldsymbol{h} -2\lambda\boldsymbol{\Psi} \textbf{K} \textbf{k} -\frac{\boldsymbol{s}}{\lambda^2} + \boldsymbol{h}, \hat{\mathbold{\varepsilon}}> = \frac{1}{dor^2}<-\frac{d^2\mathbold{S}}{d\lambda^2}\mathbold{z}  + 2\boldsymbol{h} -2\lambda\boldsymbol{\Psi} \textbf{K} \textbf{k}, \hat{\mathbold{\varepsilon}}> $\\
\\
$ [5] =  \frac{1}{dor^2}<\mathbold{p}, \frac{d\hat{\mathbold{\varepsilon}}}{d\lambda}> = \frac{1}{dor^2}<\mathbold{p},\mathbold{Q}\mathbold{p}>$\\
\\
$\implies  \frac{d^2GCV}{d\lambda^2}(\lambda) =
\\ =\frac{2s}{dor^2}\{\frac{1}{dor}[3\hat{\sigma}^2tr(\frac{d\mathbold{S}}{d\lambda}) + 4<\mathbold{p}, \hat{\mathbold{\varepsilon}}>]tr(\frac{d\mathbold{S}}{d\lambda}) + \hat{\sigma}^2tr(\frac{d^2\mathbold{S}}{d\lambda^2}) + <\mathbold{p},\mathbold{Q} \mathbold{p}> + <\frac{d\mathbold{p}}{d\lambda}, \hat{\mathbold{\varepsilon}}>\} = \\
=\frac{2s}{dor^2}\{\frac{1}{dor}[3\hat{\sigma}^2tr(\frac{d\mathbold{S}}{d\lambda}) + 4a]tr(\frac{d\mathbold{S}}{d\lambda}) + \hat{\sigma}^2tr(\frac{d^2\mathbold{S}}{d\lambda^2}) +b+c\}$

\paragraph{Useful side computations}
\begin{enumerate}
	\item $ \frac{d\mathbold{h}}{d\lambda} = -2\boldsymbol{\Psi} \textbf{T}^{-1} \textbf{R}\textbf{T}^{-1} \textbf{R}\textbf{T}^{-1} \mathbf{f} = -2\boldsymbol{\Psi} \textbf{K} \textbf{k}$
\end{enumerate}

\paragraph{Redefined factors}
\begin{enumerate}
	\item $b = <\mathbold{p},\mathbold{Q}\mathbold{p}>$
	\item $c = <\frac{d\mathbold{p}}{d\lambda}, \hat{\mathbold{\varepsilon}}> $
\end{enumerate}


\chapter{Forcing term and nonhomogeneous Dirichlet}
Define $GCV_{homo}$ the computation of the GCV in the homogeneous case
\section{GCV-I-derivative}
$ \frac{dGCV}{d\lambda}(\lambda)=\frac{d[GCV_{homo}+\frac{s}{dor^2}(||\textbf{r}(\lambda)||^2-2<\hat{\mathbold{\varepsilon}},\textbf{r}(\lambda)>)]}{d\lambda}=\frac{dGCV_{homo}}{d\lambda}+s(||\textbf{r}(\lambda)||^2-2<\hat{\mathbold{\varepsilon}},\textbf{r}(\lambda)>)\frac{d(dor^{-2})}{d\lambda}+\frac{2s}{dor^2}(<\textbf{r}(\lambda),\frac{d\textbf{r}}{d\lambda}>-<\frac{d\hat{\mathbold{\varepsilon}}}{d\lambda},\textbf{r}(\lambda)>-<\hat{\mathbold{\varepsilon}},\frac{d\textbf{r}(\lambda)}{d\lambda}>)$\\
\begin{equation}
V=\Psi^T\textbf{AQ}\Psi+\lambda \textbf{R}_1^T\textbf{R}_0^{-1}\textbf{R}_1
\end{equation}
\begin{equation}
\frac{d\textbf{V}^{-1}}{d\lambda}=-\textbf{V}^{-1}\textbf{R}_1^T\textbf{R}_0^{-1}\textbf{R}_1 \textbf{V}^{-1}
\end{equation}
\begin{equation}
\frac{d\textbf{S}}{d\lambda}=-\Psi \frac{d\textbf{V}^{-1}}{d\lambda}\Psi^T\textbf{AQ}
\end{equation}
\begin{equation}
\frac{d\textbf{r}}{d\lambda}=\frac{1}{\lambda}\textbf{r}(\lambda)+\lambda \textbf{Q}\Psi \frac{d\textbf{V}^{-1}}{d\lambda} \textbf{R}_1^T\textbf{R}_0^{-1}\textbf{u}^{*}
\end{equation}

\section{GCV-II-derivative}
\begin{align*}
\frac{d^2 GCV}{d\lambda^2}&=\frac{d^2 GCV_{homo}}{d\lambda^2}+2s(<\textbf{r}(\lambda),\frac{d\textbf{r}}{d\lambda}>-<\frac{d\hat{\mathbold{\varepsilon}}}{d\lambda},\textbf{r}(\lambda)>-<\hat{\mathbold{\varepsilon}},\frac{d\textbf{r}(\lambda)}{d\lambda}>)\frac{d(dor^{-2})}{d\lambda}+s(||\textbf{r}(\lambda)||^2\\&-2<\hat{\mathbold{\varepsilon}},\textbf{r}(\lambda)>)\frac{d^2}{d\lambda^2}(dor^{-2})+2\frac{s}{dor^2}[\ ||\frac{d\textbf{r}}{d\lambda}||^2+<\textbf{r}, \frac{d^2\textbf{r}}{d\lambda^2}>-<\frac{d^2 \hat{\mathbold{\varepsilon}}}{d\lambda}, \textbf{r}(\lambda)>-2<\frac{d\hat{\mathbold{\varepsilon}}}{d\lambda}, \frac{d\textbf{r}(\lambda)}{d\lambda}>\\&-<\hat{\mathbold{\varepsilon}}, \frac{d^2\textbf{r}}{d\lambda^2}>]\\&+2s\frac{d(dor^{-2})}{d\lambda}[<\textbf{r}(\lambda),\frac{d\textbf{r}}{d\lambda}>-<\frac{d\hat{\mathbold{\varepsilon}}}{d\lambda},\textbf{r}(\lambda)>-<\hat{\mathbold{\varepsilon}},\frac{d\textbf{r}(\lambda)}{d\lambda}>]
\end{align*}

\begin{equation}
\frac{d^2\hat{\mathbold{\varepsilon}}}{d\lambda^2}=-\textbf{Q}\frac{d^2\textbf{S}}{d\lambda^2}\textbf{z}
\end{equation}

\begin{equation}
\frac{d^2\textbf{r}}{d\lambda^2}=-\frac{1}{\lambda^2}\textbf{r}(\lambda)+\frac{1}{\lambda}\frac{d\textbf{r}}{d\lambda}+\textbf{Q}\Psi (\frac{d\textbf{V}^{-1}}{d\lambda} +\lambda \frac{d^2\textbf{V}^{-1}}{d\lambda^2})\textbf{R}_1^T\textbf{R}_0^{-1}\textbf{u}^{*}
\end{equation}

\begin{equation}
\frac{d^2\textbf{V}^{-1}}{d\lambda^2}=-\frac{d\textbf{V}^{-1}}{d\lambda}\textbf{R}_1^T\textbf{R}_0^{-1}\textbf{R}_1 \textbf{V}^{-1}-\textbf{V}^{-1}\textbf{R}_1^T\textbf{R}_0^{-1}\textbf{R}_1\frac{d\textbf{V}^{-1}}{d\lambda}
\end{equation}

\begin{equation}
\frac{d\ dor}{d\lambda}=-tr(\frac{d\textbf{S}(\lambda)}{d\lambda})
\end{equation}


\begin{equation}
\frac{d^2 dor^{-2}}{d\lambda^2}=2tr(\frac{d^2\textbf{S}(\lambda)}{d\lambda^2})dor^{-3}+6\ dor^{-4}\{tr(\frac{d\textbf{S}(\lambda)}{d\lambda})\}^2
\end{equation}


\end{document}